src/specs/UpdateTranscript.ec
@@ -1,9 +1,21 @@
+require import AllCore.
+require import List.
 require        Constants.
 require import PurePrimops.
 require import UInt256.
 require import Verifier.
 require import VerifierConsts.
 require import YulPrimops.
+
+(* Layout
+   BEGIN_SLOT     = 3 bytes  [0x0 - 0x2]
+   DST_SLOT       = 1 byte   [0x03]
+   STATE0_SLOT    = 32 bytes [0x04     - 0x23 (35)] 31
+   STATE1_SLOT    = 32 bytes [0x24(36) - 0x43 (67)] 31
+   CHALLANGE_SLOT = 32 bytes [0x44(68) - 0x64(100)] 31
+*)
+
+op keccakI : int list -> int.
 
 module UpdateTranscript = {
   proc low(value : uint256): unit = {
@@ -16,6 +28,13 @@ module UpdateTranscript = {
     Primops.mstore(TRANSCRIPT_STATE_1_SLOT, newState1);
     Primops.mstore(TRANSCRIPT_STATE_0_SLOT, newState0);
   }
+
+  proc mid(tS0 tS1 tC : int) : int * int = {
+    var state0, state1 : int;
+    state0 <- keccakI [0; tS0; tS1; tC];
+    state1 <- keccakI [1; tS0; tS1; tC];
+    return (state0, state1);
+  }
 }.
 
 lemma updateTranscript_extracted_equiv_low :
@@ -27,4 +46,176 @@ lemma updateTranscript_extracted_equiv_low :
 proof.
   proc.
   inline*. wp. skip. by progress.
+qed.
+
+lemma updateTranscript_pspec_revert :
+phoare [ UpdateTranscript.low : Primops.reverted ==> Primops.reverted ] = 1%r.
+proof. proc; inline*; wp; skip; by auto. qed.
+
+import MemoryMap PurePrimops.
+
+op updateTranscript_memory_footprint (m: mem) (c ks0 ks1 : uint256) : mem =
+let m1 = store8 m TRANSCRIPT_DST_BYTE_SLOT W256.zero in
+let m2 = store m1 TRANSCRIPT_CHALLENGE_SLOT c in 
+let m3 = store8 m2 TRANSCRIPT_DST_BYTE_SLOT W256.one in
+let m4 = store m3 TRANSCRIPT_STATE_1_SLOT ks1 in
+let m5 = store m4 TRANSCRIPT_STATE_0_SLOT ks0 in
+m5.
+
+axiom keccak256_transcript_dst0_pspec (m: mem) (s0 s1 ch : uint256):
+    (W32u8.unpack8(mload m TRANSCRIPT_DST_BYTE_SLOT)).[31] = W8.of_int 0 /\
+    mload m TRANSCRIPT_STATE_0_SLOT = s0 /\
+    mload m TRANSCRIPT_STATE_1_SLOT = s1 /\
+    mload m TRANSCRIPT_CHALLENGE_SLOT = ch =>
+    W256.to_uint (PurePrimops.keccak256_f(Array.offun
+      (fun (i: int) => m.[TRANSCRIPT_BEGIN_SLOT + (W256.of_int i)]) 100)) =
+    keccakI [0; W256.to_uint s0; W256.to_uint s1; W256.to_uint ch].
+
+axiom keccak256_transcript_dst1_pspec (m: mem) (s0 s1 ch : uint256):
+    (W32u8.unpack8(mload m TRANSCRIPT_DST_BYTE_SLOT)).[31] = W8.of_int 1 /\
+    mload m TRANSCRIPT_STATE_0_SLOT = s0 /\
+    mload m TRANSCRIPT_STATE_1_SLOT = s1 /\
+    mload m TRANSCRIPT_CHALLENGE_SLOT = ch =>
+    W256.to_uint (PurePrimops.keccak256_f(Array.offun
+      (fun (i: int) => m.[TRANSCRIPT_BEGIN_SLOT + (W256.of_int i)]) 100)) =
+    keccakI [1; W256.to_uint s0; W256.to_uint s1; W256.to_uint ch].
+  
+lemma updateTranscript_low_equiv_mid (m : mem) (
+      transcriptBeginG
+      transcriptState0G
+      transcriptState1G
+      transcriptChallangeG: int
+) :
+equiv [UpdateTranscript.low ~ UpdateTranscript.mid :
+arg{1} = W256.of_int transcriptChallangeG /\
+arg{2} = (transcriptState0G, transcriptState1G, transcriptChallangeG) /\
+Primops.memory{1} = m /\
+!Primops.reverted{1} /\
+W256.to_uint (mload m TRANSCRIPT_STATE_0_SLOT) = transcriptState0G /\
+W256.to_uint (mload m TRANSCRIPT_STATE_1_SLOT) = transcriptState1G /\
+W256.to_uint (mload m TRANSCRIPT_CHALLENGE_SLOT) = transcriptChallangeG
+==>
+!Primops.reverted{1} /\
+Primops.memory{1} = updateTranscript_memory_footprint m
+   (W256.of_int transcriptChallangeG)
+   (W256.of_int res{2}.`1)
+   (W256.of_int res{2}.`2)
+].
+proof. proc.
+pose m1 := store8 m TRANSCRIPT_DST_BYTE_SLOT W256.zero.
+seq 1 0: (
+  value{1} = (of_int transcriptChallangeG)%W256 /\
+  (tS0{2}, tS1{2}, tC{2}) =
+  (transcriptState0G, transcriptState1G, transcriptChallangeG) /\
+  !Primops.reverted{1} /\
+  to_uint (mload m TRANSCRIPT_STATE_0_SLOT) = transcriptState0G /\
+  to_uint (mload m TRANSCRIPT_STATE_1_SLOT) = transcriptState1G /\
+  to_uint (mload m TRANSCRIPT_CHALLENGE_SLOT) = transcriptChallangeG /\
+  Primops.memory{1} = m1
+).
+call{1} (ConcretePrimops.mstore8_pspec m TRANSCRIPT_DST_BYTE_SLOT W256.zero).
+skip. by progress.
+pose m2 := store m1 TRANSCRIPT_CHALLENGE_SLOT (of_int transcriptChallangeG)%W256.
+seq 1 0: (
+  value{1} = (of_int transcriptChallangeG)%W256 /\
+  (tS0{2}, tS1{2}, tC{2}) =
+  (transcriptState0G, transcriptState1G, transcriptChallangeG) /\
+  !Primops.reverted{1} /\
+  to_uint (mload m TRANSCRIPT_STATE_0_SLOT) = transcriptState0G /\
+  to_uint (mload m TRANSCRIPT_STATE_1_SLOT) = transcriptState1G /\
+  to_uint (mload m TRANSCRIPT_CHALLENGE_SLOT) = transcriptChallangeG /\
+  Primops.memory{1} = m2
+).
+call{1} (ConcretePrimops.mstore_pspec m1 TRANSCRIPT_CHALLENGE_SLOT (of_int transcriptChallangeG)%W256).
+skip. by progress. 
+
+seq 1 1: (#pre /\
+  to_uint newState0{1} = state0{2} /\
+  state0{2} = keccakI [0; tS0{2}; tS1{2}; tC{2}]).
+call{1} (ConcretePrimops.keccak256_pspec TRANSCRIPT_BEGIN_SLOT (W256.of_int 100)).
+wp. skip. progress.
+apply keccak256_transcript_dst0_pspec. progress.
+rewrite /m2 /m1 load_store_diff /TRANSCRIPT_DST_BYTE_SLOT /TRANSCRIPT_CHALLENGE_SLOT; try by progress.
+rewrite load_store8_same. smt().
+rewrite /m2 /m1. rewrite load_store_diff.
+rewrite /TRANSCRIPT_STATE_0_SLOT /TRANSCRIPT_CHALLENGE_SLOT. by progress.
+rewrite /TRANSCRIPT_STATE_0_SLOT /TRANSCRIPT_CHALLENGE_SLOT. by progress.
+apply load_store8_diff. rewrite /TRANSCRIPT_STATE_0_SLOT /TRANSCRIPT_DST_BYTE_SLOT. smt().
+rewrite /m2 /m1 load_store_diff /TRANSCRIPT_STATE_1_SLOT /TRANSCRIPT_CHALLENGE_SLOT; try by progress.
+apply load_store8_diff. rewrite /TRANSCRIPT_DST_BYTE_SLOT. smt().
+rewrite /m2 /m1 load_store_same. smt().
+
+pose m3 := store8 m2 TRANSCRIPT_DST_BYTE_SLOT W256.one.
+seq 1 0: (
+  value{1} = (of_int transcriptChallangeG)%W256 /\
+   (tS0{2}, tS1{2}, tC{2}) =
+   (transcriptState0G, transcriptState1G, transcriptChallangeG) /\
+   !Primops.reverted{1} /\
+   to_uint (mload m TRANSCRIPT_STATE_0_SLOT) = transcriptState0G /\
+   to_uint (mload m TRANSCRIPT_STATE_1_SLOT) = transcriptState1G /\
+   to_uint (mload m TRANSCRIPT_CHALLENGE_SLOT) = transcriptChallangeG /\
+  to_uint newState0{1} = state0{2} /\
+  state0{2} = keccakI [0; tS0{2}; tS1{2}; tC{2}] /\
+  Primops.memory{1} = m3
+).
+call{1} (ConcretePrimops.mstore8_pspec m2 TRANSCRIPT_DST_BYTE_SLOT W256.one).
+skip. by progress.
+
+seq 1 1: (#pre /\
+  to_uint newState1{1} = state1{2} /\
+  state1{2} = keccakI [1; tS0{2}; tS1{2}; tC{2}]).
+call{1} (ConcretePrimops.keccak256_pspec TRANSCRIPT_BEGIN_SLOT (W256.of_int 100)).
+wp. skip. progress.
+apply keccak256_transcript_dst1_pspec. progress.
+rewrite /m3 /m2 /m1 load_store8_same. smt().
+rewrite /m3 /m2 /m1 load_store8_diff /TRANSCRIPT_STATE_0_SLOT /TRANSCRIPT_DST_BYTE_SLOT. smt().
+rewrite load_store_diff /TRANSCRIPT_CHALLENGE_SLOT. by progress. by progress.
+rewrite load_store8_diff; smt().
+rewrite /m3 /m2 /m1 load_store8_diff /TRANSCRIPT_STATE_1_SLOT /TRANSCRIPT_DST_BYTE_SLOT. smt().
+rewrite load_store_diff /TRANSCRIPT_CHALLENGE_SLOT; try by progress.
+rewrite load_store8_diff; smt().
+rewrite /m3 /m2 /m1 load_store8_diff /TRANSCRIPT_CHALLENGE_SLOT /TRANSCRIPT_DST_BYTE_SLOT. smt().
+rewrite load_store_same. smt().
+
+exists* newState1{1}. elim*=> ns1.
+pose m4 := store m3 TRANSCRIPT_STATE_1_SLOT ns1.
+seq 1 0:(
+  ns1 = newState1{1} /\  
+  value{1} = (of_int transcriptChallangeG)%W256 /\
+   (tS0{2}, tS1{2}, tC{2}) =
+   (transcriptState0G, transcriptState1G, transcriptChallangeG) /\
+   !Primops.reverted{1} /\
+   to_uint (mload m TRANSCRIPT_STATE_0_SLOT) = transcriptState0G /\
+   to_uint (mload m TRANSCRIPT_STATE_1_SLOT) = transcriptState1G /\
+   to_uint (mload m TRANSCRIPT_CHALLENGE_SLOT) = transcriptChallangeG /\
+   to_uint newState0{1} = state0{2} /\
+   state0{2} = keccakI [0; tS0{2}; tS1{2}; tC{2}] /\
+  to_uint newState1{1} = state1{2} /\
+   state1{2} = keccakI [1; tS0{2}; tS1{2}; tC{2}] /\
+   Primops.memory{1} = m4
+).
+call{1} (ConcretePrimops.mstore_pspec m3 TRANSCRIPT_STATE_1_SLOT ns1).
+skip. by progress.
+
+exists* newState0{1}. elim*=> ns0.
+pose m5 := store m4 TRANSCRIPT_STATE_0_SLOT ns0.
+seq 1 0:(
+  ns1 = newState1{1} /\ ns0 = newState0{1} /\  
+  value{1} = (of_int transcriptChallangeG)%W256 /\
+   (tS0{2}, tS1{2}, tC{2}) =
+   (transcriptState0G, transcriptState1G, transcriptChallangeG) /\
+   !Primops.reverted{1} /\
+   to_uint (mload m TRANSCRIPT_STATE_0_SLOT) = transcriptState0G /\
+   to_uint (mload m TRANSCRIPT_STATE_1_SLOT) = transcriptState1G /\
+   to_uint (mload m TRANSCRIPT_CHALLENGE_SLOT) = transcriptChallangeG /\
+   to_uint newState0{1} = state0{2} /\
+   state0{2} = keccakI [0; tS0{2}; tS1{2}; tC{2}] /\
+  to_uint newState1{1} = state1{2} /\
+   state1{2} = keccakI [1; tS0{2}; tS1{2}; tC{2}] /\
+   Primops.memory{1} = m5
+).
+call{1} (ConcretePrimops.mstore_pspec m4 TRANSCRIPT_STATE_0_SLOT ns0).
+skip. by progress.
+
+skip. by progress.
 qed.
